CrSymbolicSemantics.v
@@ -1,38 +1,40 @@
 From MyProject Require Import CrTransformer.
 From MyProject Require Import CrIdentifiers.
-From MyProject Require Import CrConcreteSemantics.
+From MyProject Require Import CrSemantics.
 From MyProject Require Import SmtExpr.
 From MyProject Require Import StringUtils.
 Require Import ZArith.
 Require Import Coq.Strings.String.
 
 (* Convert FunctionArgument to SmtExpr *)
-Definition function_argument_to_smt (arg : FunctionArgument) : SmtExpr :=
-    match arg with
-    | HeaderArg (HeaderCtr h) => SmtVar ("hdr_" ++ h)
-    | CtrlPlaneArg (CtrlPlaneConfigNameCtr c) => SmtVar ("ctrl_" ++ c)
-    | ConstantArg n => SmtConst n
-    | StatefulArg (StateVarCtr s) => SmtVar ("state_" ++ s)
-    end.
+Definition lookup_smt (arg : FunctionArgument) (ps : ProgramState SmtExpr) : SmtExpr :=
+  match arg with
+  | CtrlPlaneArg c => ctrl_plane_map SmtExpr ps c
+  | HeaderArg h    => header_map SmtExpr ps h
+  | ConstantArg n  => SmtConst n
+  | StatefulArg s  => state_var_map SmtExpr ps s
+  end.
 
 (* Define the symbolic interpreter for header operation expressions *)
-Definition eval_hdr_op_expr_smt (h : HdrOp) : SmtExpr :=
+Definition eval_hdr_op_expr_smt (h : HdrOp) (ps : ProgramState SmtExpr) : SmtExpr :=
     match h with
     | StatefulOp f arg1 arg2 _ =>
        match f with 
-         | AddOp => SmtBitAdd (function_argument_to_smt arg1) (function_argument_to_smt arg2)
+         | AddOp => SmtBitAdd (lookup_smt arg1 ps) (lookup_smt arg2 ps)
        end
     | StatelessOp f arg1 arg2 _ =>
        match f with
-         | AddOp => SmtBitAdd (function_argument_to_smt arg1) (function_argument_to_smt arg2)
+         | AddOp => SmtBitAdd (lookup_smt arg1 ps) (lookup_smt arg2 ps)
        end
     end.
 
-Definition eval_hdr_op_smt (h : HdrOp) : SmtExpr :=
-    match h with
-    | StatefulOp f arg1 arg2 target => SmtBitEq (function_argument_to_smt (StatefulArg target)) (eval_hdr_op_expr_smt h)
-    | StatelessOp f arg1 arg2 target => SmtBitEq (function_argument_to_smt (HeaderArg target)) (eval_hdr_op_expr_smt h)
-    end.
+Definition eval_hdr_op_smt_assign (ho : HdrOp) (ps: ProgramState SmtExpr) : ProgramState SmtExpr :=
+    match ho with
+    | StatefulOp f arg1 arg2 target =>
+        let op_output := eval_hdr_op_expr_smt ho ps in update_state ps target op_output
+    | StatelessOp f arg1 arg2 target => 
+        let op_output := eval_hdr_op_expr_smt ho ps in update_hdr ps target op_output
+    end.  
 
 (* Convert ProgramState to SMT Valuation *)
 Definition prog_state_to_smt_val (ps: ProgramState uint8) : SmtValuation :=
@@ -49,3 +51,14 @@ Definition prog_state_to_smt_val (ps: ProgramState uint8) : SmtValuation :=
          Why does this even work?
          I guess because cr_val_to_sml is only ever applied to the smt_transformed formula,
         not arbitrary ones? *)
+
+Instance Semantics_SmtExpr : Semantics SmtExpr := {
+  (* Function to lookup arg in program state *)
+  lookup_function_argument := lookup_smt;
+
+  (* Function to evaluate header operation expression *)
+  eval_hdr_op_expr := eval_hdr_op_expr_smt;
+
+  (* Function to update header or state variable in program state *)
+  eval_hdr_op_assign := eval_hdr_op_smt_assign;
+}.
